src/tools/parallelcomposition/translateTosapic/translate_to_sapicScript.sml
@@ -618,122 +618,263 @@ ASM_SIMP_TAC (srw_ss()) [] >>
 
 
 
-
-
+*)
+val symbtree_to_sapic_single_step_simulation_thm = store_thm(
+  "symbtree_to_sapic_single_step_simulation_thm",
+  ``
 ∀E Tree Tree' Pro i Re NRe.
         (((single_step_execute_symbolic_tree Tree E Tree' ) ∧ (sim Tree (Pconfig (Pro,i,Re,NRe))))
-        ⇒ (∃Pro' i' Re' NRe' Ev. (sim Tree' (Pconfig (Pro',i',Re',NRe'))) ∧ (sapic_position_transition (Pconfig (Pro,i,Re,NRe)) Ev (Pconfig (Pro',i',Re',NRe')))))
-
+         ⇒ (∃Pro' i' Re' NRe' Ev. (sim Tree' (Pconfig (Pro',i',Re',NRe'))) ∧ (sapic_position_transition (Pconfig (Pro,i,Re,NRe)) Ev (Pconfig (Pro',i',Re',NRe')))))``,                                                                                                               
 gen_tac >>
-Cases_on ‘E’
+Cases_on ‘E’ >- (
 rw[single_step_execute_symbolic_tree_def]>>
 IMP_RES_TAC sim_def>>
 ASM_SIMP_TAC (srw_ss()) [symbtree_to_sapic_def,position_in_tree_def] >>
 ASM_SIMP_TAC (srw_ss()) [sapic_position_transition_def]>>
 ASM_SIMP_TAC (srw_ss()) [sapic_position_out_transition_def]>>
-Q.EXISTS_TAC `symbtree_to_sapic Tree'` >> Q.EXISTS_TAC `i'+1` >> Q.EXISTS_TAC `Re` >> Q.EXISTS_TAC `NRe` >>  Q.EXISTS_TAC `[Fact OutFact [translate_birexp_to_sapicterm (BExp_Den b)]]`>>
-rw[sim_def] >>
+Q.EXISTS_TAC `symbtree_to_sapic Tree'` >>
+Q.EXISTS_TAC `i'+1` >>
+Q.EXISTS_TAC `Re` >>
+Q.EXISTS_TAC `NRe` >>
+Q.EXISTS_TAC `[Fact OutFact [translate_birexp_to_sapicterm (BExp_Den b)]]`>>
+rw[sim_def] >-(
 IMP_RES_TAC position_of_val_thm>>
-ASM_SIMP_TAC (srw_ss()) []>>
+ASM_SIMP_TAC (srw_ss()) []
+)>>
 IMP_RES_TAC env_of_val_thm>>
 rewrite_tac[env_of_tree_def]>>
 ASM_SIMP_TAC (srw_ss()) []
-
+)
 (*end of P2A*)
-             
+>-(            
 rw[single_step_execute_symbolic_tree_def]>>
 IMP_RES_TAC sim_def>>
 ASM_SIMP_TAC (srw_ss()) [symbtree_to_sapic_def,position_in_tree_def,sapic_position_transition_def]>>
 ASM_SIMP_TAC (srw_ss()) [sapic_position_in_transition_def]>>
-Cases_on ‘H’ >> Cases_on ‘Re’
-rewrite_tac[sapic_renaming_update_def]
-Q.EXISTS_TAC `symbtree_to_sapic Tree'` >> Q.EXISTS_TAC `i'+1` >> Q.EXISTS_TAC `Renaming
-             f'⦇Var "Adv" 0 ↦ SOME (TVar (translate_birvar_to_sapicvar b))⦈` >> Q.EXISTS_TAC `NRe` >>  Q.EXISTS_TAC `[Fact InFact [TVar (translate_birvar_to_sapicvar b)]]`>>
-rw[sim_def] >>
-IMP_RES_TAC position_of_val_thm
+Cases_on ‘H’ >-(
+Cases_on ‘Re’ >-(
+rewrite_tac[sapic_renaming_update_def] >>
+Q.EXISTS_TAC `symbtree_to_sapic Tree'` >>
+Q.EXISTS_TAC `i'+1` >>
+Q.EXISTS_TAC `Renaming f'⦇Var "Adv" 0 ↦ SOME (TVar (translate_birvar_to_sapicvar b))⦈` >>
+Q.EXISTS_TAC `NRe` >>
+Q.EXISTS_TAC `[Fact InFact [TVar (translate_birvar_to_sapicvar b)]]`>>
+rw[sim_def] >-(
+IMP_RES_TAC position_of_val_thm >>
 ASM_SIMP_TAC (srw_ss()) []
-
-IMP_RES_TAC env_of_val_thm
-FULL_SIMP_TAC (list_ss++pred_setSimps.PRED_SET_ss++boolSimps.LIFT_COND_ss++boolSimps.EQUIV_EXTRACT_ss) [sapic_renaming_update_def,symb_interpr_dom_def,sapic_renaming_dom_def,symb_interpr_update_def,env_of_tree_def,IMAGE_DEF,EXTENSION]
-gen_tac
-PAT_X_ASSUM ``!x. A `` (ASSUME_TAC o (Q.SPECL [`x`]))
-rw[UPDATE_def]
-Q.EXISTS_TAC `BVar "Adv" (BType_Imm Bit64)`
+)
+>-(
+IMP_RES_TAC env_of_val_thm >>
+FULL_SIMP_TAC (list_ss++pred_setSimps.PRED_SET_ss++boolSimps.LIFT_COND_ss++boolSimps.EQUIV_EXTRACT_ss) [sapic_renaming_update_def,symb_interpr_dom_def,sapic_renaming_dom_def,symb_interpr_update_def,env_of_tree_def,IMAGE_DEF,EXTENSION]>>
+gen_tac >>
+PAT_X_ASSUM ``!x. A `` (ASSUME_TAC o (Q.SPECL [`x`]))>>
+rw[UPDATE_def]>-(
+Q.EXISTS_TAC `BVar "Adv" (BType_Imm Bit64)`>>
 FULL_SIMP_TAC (list_ss++pred_setSimps.PRED_SET_ss++boolSimps.LIFT_COND_ss++boolSimps.EQUIV_EXTRACT_ss) [translate_birvar_to_sapicvar_def]
-
-
-eq_tac
-
-rpt strip_tac
-Q.EXISTS_TAC `x'`                        
+)>>
+eq_tac >-(
+rpt strip_tac >>
+Q.EXISTS_TAC `x'` >>                       
+ASM_SIMP_TAC (srw_ss()) []>>
+Cases_on ‘x' = BVar "Adv" (BType_Imm Bit64)’>>
 ASM_SIMP_TAC (srw_ss()) []
-Cases_on ‘x' = BVar "Adv" (BType_Imm Bit64)’
-ASM_SIMP_TAC (srw_ss()) []
-
-ASM_SIMP_TAC (srw_ss()) []
-
-
-rpt strip_tac
-Q.EXISTS_TAC `x'`                        
-ASM_SIMP_TAC (srw_ss()) []
-Cases_on ‘x' = BVar "Adv" (BType_Imm Bit64)’
+) >>
+rpt strip_tac >>
+Q.EXISTS_TAC `x'` >>                        
+ASM_SIMP_TAC (srw_ss()) [] >>
+Cases_on ‘x' = BVar "Adv" (BType_Imm Bit64)’ >>
 FULL_SIMP_TAC (list_ss++pred_setSimps.PRED_SET_ss++boolSimps.LIFT_COND_ss++boolSimps.EQUIV_EXTRACT_ss) [translate_birvar_to_sapicvar_def]
-
-FULL_SIMP_TAC (list_ss++pred_setSimps.PRED_SET_ss++boolSimps.LIFT_COND_ss++boolSimps.EQUIV_EXTRACT_ss) [translate_birvar_to_sapicvar_def]              
-
-
-
-
+))))
 (*end of A2P*)
-
-
+>-( 
 rw[single_step_execute_symbolic_tree_def]>>
 IMP_RES_TAC sim_def>>
 ASM_SIMP_TAC (srw_ss()) [symbtree_to_sapic_def,position_in_tree_def,sapic_position_transition_def]>>
 ASM_SIMP_TAC (srw_ss()) [sapic_position_new_transition_def]>>
-Cases_on ‘H’ >> Cases_on ‘Re’ >> Cases_on ‘NRe’ >>
-rewrite_tac[sapic_renaming_update_def,sapic_name_renaming_update_def]
-Q.EXISTS_TAC `symbtree_to_sapic Tree'` >> Q.EXISTS_TAC `i'+1` >> Q.EXISTS_TAC `Renaming f'⦇Var "RNG" 0 ↦SOME (Con (translate_birvar_to_sapicfreshname b))⦈` >> Q.EXISTS_TAC `NameRenaming f''⦇translate_birvar_to_sapicfreshname b ↦SOME (Con (translate_birvar_to_sapicfreshname b))⦈` >>  Q.EXISTS_TAC `[]`>>
-rw[sim_def] >>
-IMP_RES_TAC position_of_val_thm
+Cases_on ‘H’ >-(
+Cases_on ‘Re’ >-(
+Cases_on ‘NRe’ >-(
+rewrite_tac[sapic_renaming_update_def,sapic_name_renaming_update_def] >>
+Q.EXISTS_TAC `symbtree_to_sapic Tree'` >>
+Q.EXISTS_TAC `i'+1` >>
+Q.EXISTS_TAC `Renaming f'⦇Var "RNG" 0 ↦SOME (Con (translate_birvar_to_sapicfreshname b))⦈` >>
+Q.EXISTS_TAC `NameRenaming f''⦇translate_birvar_to_sapicfreshname b ↦SOME (Con (translate_birvar_to_sapicfreshname b))⦈` >>
+Q.EXISTS_TAC `[]`>>
+rw[sim_def] >-(
+IMP_RES_TAC position_of_val_thm>>
 ASM_SIMP_TAC (srw_ss()) []
-
-IMP_RES_TAC env_of_val_thm
-FULL_SIMP_TAC (list_ss++pred_setSimps.PRED_SET_ss++boolSimps.LIFT_COND_ss++boolSimps.EQUIV_EXTRACT_ss) [sapic_renaming_update_def,symb_interpr_dom_def,sapic_renaming_dom_def,symb_interpr_update_def,env_of_tree_def,IMAGE_DEF,EXTENSION]
-gen_tac
-PAT_X_ASSUM ``!x. A `` (ASSUME_TAC o (Q.SPECL [`x`]))
-rw[UPDATE_def]
-Q.EXISTS_TAC `BVar "RNG" (BType_Imm Bit64)`
+)
+>-(
+IMP_RES_TAC env_of_val_thm>>
+FULL_SIMP_TAC (list_ss++pred_setSimps.PRED_SET_ss++boolSimps.LIFT_COND_ss++boolSimps.EQUIV_EXTRACT_ss) [sapic_renaming_update_def,symb_interpr_dom_def,sapic_renaming_dom_def,symb_interpr_update_def,env_of_tree_def,IMAGE_DEF,EXTENSION]>>
+gen_tac>>
+PAT_X_ASSUM ``!x. A `` (ASSUME_TAC o (Q.SPECL [`x`]))>>
+rw[UPDATE_def]>-(
+Q.EXISTS_TAC `BVar "RNG" (BType_Imm Bit64)`>>
 FULL_SIMP_TAC (list_ss++pred_setSimps.PRED_SET_ss++boolSimps.LIFT_COND_ss++boolSimps.EQUIV_EXTRACT_ss) [translate_birvar_to_sapicvar_def]
-
-
-eq_tac
-
-rpt strip_tac
-Q.EXISTS_TAC `x'`                        
+)>>
+eq_tac >-(
+rpt strip_tac >>
+Q.EXISTS_TAC `x'` >>                         
+ASM_SIMP_TAC (srw_ss()) [] >>
+Cases_on ‘x' = BVar "RNG" (BType_Imm Bit64)’ >>
 ASM_SIMP_TAC (srw_ss()) []
-Cases_on ‘x' = BVar "RNG" (BType_Imm Bit64)’
-ASM_SIMP_TAC (srw_ss()) []
-
-ASM_SIMP_TAC (srw_ss()) []
-
-
-rpt strip_tac
-Q.EXISTS_TAC `x'`                        
-ASM_SIMP_TAC (srw_ss()) []
-Cases_on ‘x' = BVar "RNG" (BType_Imm Bit64)’
+) >>
+rpt strip_tac >>
+Q.EXISTS_TAC `x'` >>                       
+ASM_SIMP_TAC (srw_ss()) [] >>
+Cases_on ‘x' = BVar "RNG" (BType_Imm Bit64)’>>
 FULL_SIMP_TAC (list_ss++pred_setSimps.PRED_SET_ss++boolSimps.LIFT_COND_ss++boolSimps.EQUIV_EXTRACT_ss) [translate_birvar_to_sapicvar_def]
-
-FULL_SIMP_TAC (list_ss++pred_setSimps.PRED_SET_ss++boolSimps.LIFT_COND_ss++boolSimps.EQUIV_EXTRACT_ss) [translate_birvar_to_sapicvar_def]   
-
-
+)))))
 (*end of Sync_Fr*)
+>-(
+rw[single_step_execute_symbolic_tree_def]>>
+IMP_RES_TAC sim_def>>
+ASM_SIMP_TAC (srw_ss()) [symbtree_to_sapic_def,position_in_tree_def] >>
+ASM_SIMP_TAC (srw_ss()) [sapic_position_transition_def]>>
+ASM_SIMP_TAC (srw_ss()) [sapic_position_event_transition_def]>>
+Q.EXISTS_TAC `symbtree_to_sapic Tree'` >>
+Q.EXISTS_TAC `i'+1` >>
+Q.EXISTS_TAC `Re` >>
+Q.EXISTS_TAC `NRe` >>
+Q.EXISTS_TAC `[Fact TermFact [translate_birexp_to_sapicterm (BExp_Den b)]]`>>
+rw[sim_def] >-(
+IMP_RES_TAC position_of_val_thm>>
+ASM_SIMP_TAC (srw_ss()) []
+)>>
+IMP_RES_TAC env_of_val_thm>>
+rewrite_tac[env_of_tree_def]>>
+ASM_SIMP_TAC (srw_ss()) []
+)
+(*end of Event*)
+>-(
+rw[single_step_execute_symbolic_tree_def]>>
+IMP_RES_TAC sim_def>>
+ASM_SIMP_TAC (srw_ss()) [symbtree_to_sapic_def,position_in_tree_def,sapic_position_transition_def]>>
+ASM_SIMP_TAC (srw_ss()) [sapic_position_let_true_transition_def,sapic_position_let_false_transition_def]>>
+Cases_on ‘H’ >>
+Cases_on ‘Re’ >>
+Cases_on ‘NRe’ >>
+rewrite_tac[sapic_renaming_update_def,sapic_name_renaming_update_def] >>
+Q.EXISTS_TAC `symbtree_to_sapic Tree'` >>
+Q.EXISTS_TAC `i'+1` >>
+Q.EXISTS_TAC ` Renaming f'⦇Var "crypto" 0 ↦ SOME (translate_birexp_to_sapicterm (BExp_Den b))⦈ ` >>
+Q.EXISTS_TAC `NameRenaming f''` >>
+Q.EXISTS_TAC `[]`>>
+rw[sim_def] >-(
+IMP_RES_TAC position_of_val_thm>>
+ASM_SIMP_TAC (srw_ss()) []
+)
+>-(
+IMP_RES_TAC env_of_val_thm>>
+FULL_SIMP_TAC (list_ss++pred_setSimps.PRED_SET_ss++boolSimps.LIFT_COND_ss++boolSimps.EQUIV_EXTRACT_ss) [sapic_renaming_update_def,symb_interpr_dom_def,sapic_renaming_dom_def,symb_interpr_update_def,env_of_tree_def,IMAGE_DEF,EXTENSION]>>
+gen_tac >>
+PAT_X_ASSUM ``!x. A `` (ASSUME_TAC o (Q.SPECL [`x`]))>>
+rw[UPDATE_def]>-(
+Q.EXISTS_TAC `BVar "crypto" (BType_Imm Bit64)`>>
+FULL_SIMP_TAC (list_ss++pred_setSimps.PRED_SET_ss++boolSimps.LIFT_COND_ss++boolSimps.EQUIV_EXTRACT_ss) [translate_birvar_to_sapicvar_def]
+)>>
+eq_tac >-(
+rpt strip_tac >>
+Q.EXISTS_TAC `x'` >>                       
+ASM_SIMP_TAC (srw_ss()) []>>
+Cases_on ‘x' = BVar "crypto" (BType_Imm Bit64)’>>
+ASM_SIMP_TAC (srw_ss()) []
+)>>
+rpt strip_tac >>
+Q.EXISTS_TAC `x'`  >>                      
+ASM_SIMP_TAC (srw_ss()) []>>
+Cases_on ‘x' = BVar "crypto" (BType_Imm Bit64)’>>
+FULL_SIMP_TAC (list_ss++pred_setSimps.PRED_SET_ss++boolSimps.LIFT_COND_ss++boolSimps.EQUIV_EXTRACT_ss) [translate_birvar_to_sapicvar_def]
+))
+(*end of Crypto*)
+>-(
+rw[single_step_execute_symbolic_tree_def]>>
+IMP_RES_TAC sim_def>>
+ASM_SIMP_TAC (srw_ss()) [symbtree_to_sapic_def,position_in_tree_def] >>
+ASM_SIMP_TAC (srw_ss()) [sapic_position_transition_def]>>
+ASM_SIMP_TAC (srw_ss()) [sapic_position_replication_transition_def]>>
+Q.EXISTS_TAC `symbtree_to_sapic Tree'` >>
+Q.EXISTS_TAC `i'+1` >>
+Q.EXISTS_TAC `Re` >>
+Q.EXISTS_TAC `NRe` >>
+Q.EXISTS_TAC `[]`>>
+rw[sim_def] >-(
+IMP_RES_TAC position_of_val_thm>>
+ASM_SIMP_TAC (srw_ss()) []
+)>>
+IMP_RES_TAC env_of_val_thm>>
+rewrite_tac[env_of_tree_def]>>
+ASM_SIMP_TAC (srw_ss()) []
+)
+(*end of Loop*)      
+>-(              
+rw[single_step_execute_symbolic_tree_def]
+>-(
+IMP_RES_TAC sim_def>>
+ASM_SIMP_TAC (srw_ss()) [symbtree_to_sapic_def,position_in_tree_def] >>
+ASM_SIMP_TAC (srw_ss()) [sapic_position_transition_def]>>
+ASM_SIMP_TAC (srw_ss()) [sapic_position_conditional_false_transition_def,sapic_position_conditional_true_transition_def]>>
+Q.EXISTS_TAC `symbtree_to_sapic Tree'` >>
+Q.EXISTS_TAC `i'+1` >>
+Q.EXISTS_TAC `Re` >>
+Q.EXISTS_TAC `NRe` >>
+Q.EXISTS_TAC `[]`>>
+rw[sim_def] >-(
+IMP_RES_TAC position_of_val_thm>>
+ASM_SIMP_TAC (srw_ss()) []
+)>>
+IMP_RES_TAC env_of_val_thm>>
+rewrite_tac[env_of_tree_def]>>
+ASM_SIMP_TAC (srw_ss()) []
+)
+>-(
+IMP_RES_TAC sim_def>>
+ASM_SIMP_TAC (srw_ss()) [symbtree_to_sapic_def,position_in_tree_def] >>
+ASM_SIMP_TAC (srw_ss()) [sapic_position_transition_def]>>
+ASM_SIMP_TAC (srw_ss()) [sapic_position_conditional_false_transition_def,sapic_position_conditional_true_transition_def]>>
+Q.EXISTS_TAC `symbtree_to_sapic Tree'` >>
+Q.EXISTS_TAC `i'+1` >>
+Q.EXISTS_TAC `Re` >>
+Q.EXISTS_TAC `NRe` >>
+Q.EXISTS_TAC `[]`>>
+rw[sim_def] >-(
+IMP_RES_TAC position_of_val_thm>>
+ASM_SIMP_TAC (srw_ss()) []
+)>>
+IMP_RES_TAC env_of_val_thm>>
+rewrite_tac[env_of_tree_def]>>
+ASM_SIMP_TAC (srw_ss()) []             
+))
+(*end of Branch *)  
+>-(
+rw[single_step_execute_symbolic_tree_def]>>
+IMP_RES_TAC sim_def>>
+ASM_SIMP_TAC (srw_ss()) [symbtree_to_sapic_def,position_in_tree_def] >>
+ASM_SIMP_TAC (srw_ss()) [sapic_position_transition_def]>>
+Q.EXISTS_TAC `symbtree_to_sapic Tree'` >>
+Q.EXISTS_TAC `i'` >>
+Q.EXISTS_TAC `Re` >>
+Q.EXISTS_TAC `NRe` >>
+Q.EXISTS_TAC `[]`>>
+rw[sim_def] >-(
+IMP_RES_TAC position_of_val_thm>>
+ASM_SIMP_TAC (srw_ss()) []
+)>>
+IMP_RES_TAC env_of_val_thm>>
+rewrite_tac[env_of_tree_def]>>
+ASM_SIMP_TAC (srw_ss()) []
+)
+(*end of silent *)
+);
 
 
 
+
+
+(*
 
               
-
 IMP_RES_TAC EQ_IMP_THM      
 IMP_RES_TAC AND_INTRO_THM                             
 PAT_X_ASSUM ``!x'. A `` (ASSUME_TAC o (Q.SPECL [`BVar "Adv" (BType_Imm Bit64)`]))
